\documentclass{article}

\usepackage{amsfonts}
\usepackage{amsmath}
\usepackage{amssymb}
\usepackage{amsthm}
\usepackage{caption}
\usepackage{color}
\usepackage{enumerate}
\usepackage{fancyhdr}
\usepackage{hyperref}
\usepackage{graphicx}
\usepackage{latexsym}
\usepackage{listings}
\usepackage{mathrsfs}
\usepackage{natbib}
\usepackage[nottoc]{tocbibind}
\usepackage{url}

\providecommand{\all}{\ \forall \ }
\providecommand{\bs}{\backslash}
\providecommand{\e}{\varepsilon}
\providecommand{\E}{\ \exists \ }
\providecommand{\lm}[2]{\lim_{#1 \rightarrow #2}}
\providecommand{\m}[1]{\mathbb{#1}}
\providecommand{\nv}{{}^{-1}}
\providecommand{\ov}[1]{\overline{#1}}
\providecommand{\p}{\newpage}
\providecommand{\q}{$\quad$ \newline}
\providecommand{\rt}{\rightarrow}
\providecommand{\Rt}{\Rightarrow}
\providecommand{\vc}[1]{\boldsymbol{#1}}
\providecommand{\wh}[1]{\widehat{#1}}

\begin{document}
\begin{flushleft}

\section{Gamma and Inverse-Gamma}

\begin{align*}
\text{Gamma}(x \mid \text{shape} = \alpha, \text{rate} = \beta) &= \frac{\beta^\alpha}{\Gamma(\alpha)} x^{\alpha - 1} e^{- \beta x} \\
\end{align*}

Let $y = x \nv = g(x)$ so that $g \nv (y) = y \nv $ and $\frac{d g \nv}{d y} \mid_y  = - y^{-2}$. Then, we apply the transformation:

\begin{align*}
p( x \nv = y \mid  \alpha, \beta) &= p(x = g \nv (y) \mid \alpha, \beta) \left | \frac{d g \nv}{d y} \right |_y \\
&= \frac{\beta^\alpha}{\Gamma(\alpha)} (y \nv)^{\alpha - 1} e^{- \beta (y \nv)} |- y^{-2}| \\
&= \frac{\beta^\alpha}{\Gamma(\alpha)} y ^{-(\alpha + 1)} e^{- \beta/y}
\end{align*}

Hence, the pdf of the Inverse-Gamma distribution is:

\begin{align*}
\text{Inv-Gamma}(x \mid \text{shape} = \alpha, \text{rate} = \beta) &= \frac{\beta^\alpha}{\Gamma(\alpha)} x^{-(\alpha + 1)} e^{- \beta / x}
\end{align*}

\end{flushleft}
\end{document}